Table/BuiltinExtensions/Numeric.lean
@@ -22,9 +22,11 @@ theorem Int.natAbs_of_nonneg_eq_toNat : ∀ z : Int, z ≥ 0 → z.natAbs = z.to
 theorem Int.add_neg_eq_sub (m : Int) : ∀ n, n < 0 → m + n = m - n.natAbs
   | negSucc n, h => rfl
 
-
 -- -- TODO: decide whether to use this or `Fin.instOfNat`
 -- instance (k : Nat) : OfNat (Fin k.succ) n :=
 --   if h : n < k.succ
 --   then ⟨n, h⟩
 --   else ⟨0, Nat.zero_lt_succ k⟩
+
+abbrev DecidableLE (τ : Type _) [LE τ] :=
+  DecidableRel (· ≤ · : τ → τ → Prop)
