Table/BuiltinExtensions.lean
@@ -1,5 +1,3 @@
-import Table.BuiltinExtensions.Logic
-import Table.BuiltinExtensions.Numeric
 import Table.BuiltinExtensions.List.Basic
 import Table.BuiltinExtensions.List.Counts
 import Table.BuiltinExtensions.List.Filtering
@@ -7,3 +5,5 @@ import Table.BuiltinExtensions.List.GroupPairsByKey
 import Table.BuiltinExtensions.List.MergeSort
 import Table.BuiltinExtensions.List.Predicates
 import Table.BuiltinExtensions.List.Sieve
+import Table.BuiltinExtensions.Logic
+import Table.BuiltinExtensions.Numeric
